hashtbl/WhoHashtbl.v
@@ -18,7 +18,70 @@ Fixpoint find (a : Type) (k : hashkey) (l : hl a) {struct l} :=
         find k xs
   end.
 
+Definition is_hashtbl a  (h : ht a) :=
+  forall k v i, 
+    0 < len h /\
+    (0 <= i /\ i < len h ->
+    In (k,v) (get i h) ->
+    mod (hash k) (len h) = i).
+
 Definition repr (a : Type) (h : ht a) (l : hl a) :=
-  forall k v i, In (k,v) (get i h) -> 
-    find k (get i h) = find k l.
+  is_hashtbl h /\
+  forall k, find k (get (mod (hash k) (len h)) h) = find k l.
+
+Lemma mod_lt :
+  forall i m,
+    0 < m -> mod i m < m.
+Proof.
+  intros i m L.
+  assert (m > 0) by omega.
+  exact (proj2 (Z_mod_lt i m H)).
+Qed.
+  
+Lemma find_cons : 
+  forall a l1 l2 k k' (v : a),
+    find k l1 = find k l2 ->
+    find k ((k',v)::l1) = find k ((k',v)::l2).
+Proof.
+  intros a l1 l2 k k' v EQ; simpl; rewrite EQ; auto.
+Qed.
+
+Lemma add_elem : 
+  forall a (h : ht a) i k v,
+    is_hashtbl h -> i = mod (hash k) (len h) ->
+      is_hashtbl (set i (cons (k,v) (get i h)) h).
+Proof.
+  unfold is_hashtbl, repr in *; 
+    intros a h i k v IH IM k0 v0 i0. 
+  assert (0 < len h) by (apply (IH k v i)).
+  rewrite <- update_len in *; split; auto.
+  intros ENCL LIN.
+  case_eq (Z_eq_dec i i0); intros E D.
+  rewrite E in *; clear E D. rewrite get_set_eq in LIN.
+  generalize (in_inv LIN); intros [K | K]. injection K as K1 K2; rewrite K1, K2 in *; clear K1 K2 K. auto. 
+  apply (IH k0 v0 i0) ; auto. intuition. 
+  rewrite get_set_neq in LIN; auto. apply (IH k0 v0 i0); auto. 
+  intuition. rewrite IM; apply mod_lt; auto. 
+Qed.
+
+Lemma add_elem2 : 
+  forall a (h : ht a) l i k v,
+    is_hashtbl h -> repr h l -> i = mod (hash k) (len h) ->
+      repr (set i (cons (k,v) (get i h)) h) (cons (k,v) l).
+Proof.
+  unfold is_hashtbl, repr; 
+  intros a h l i key v IH [R1 R2] IM. split.
+  apply add_elem; auto. intros k0.
+  rewrite <- update_len in *. rewrite IM in *; clear IM.
+  assert (GZ : 0 < len h) by (apply (IH key v i)).
+  assert (LT : mod (hash k0) (len h) < len h ) by ( apply mod_lt; auto).
+  case_eq (Z_eq_dec (mod (hash k0) (len h)) (mod (hash key) (len h))); intros E D.
+  rewrite <- E in *; clear E D; rewrite get_set_eq in *; auto.
+  apply find_cons; apply R2. 
+  rewrite get_set_neq; auto.
+  simpl. case_eq (h_eq_dec k0 key); intros; auto. congruence.
+  apply mod_lt; auto.
+Qed.
+
+  
 
