coq_files/WhoArray.v
@@ -5,20 +5,20 @@ Parameter get: forall (a2 : Type)  , int -> array a2 -> a2.
 
 Parameter set: 
   forall (a3 : Type)  , int -> a3 -> array a3 -> array a3.
-Parameter length: forall (a4 : Type)  , array a4 -> int.
+Parameter len: forall (a4 : Type)  , array a4 -> int.
 
-Axiom update_length: 
+Axiom update_len: 
   forall (a5 : Type) (t:array a5) (i4:int) (z:a5), 
-    length t = length (set i4 z t).
+    len t = len (set i4 z t).
 
 Axiom get_set_eq: 
   forall (a6 : Type) (t1:array a6) (i5:int) (z1:a6),
-         i5 < length t1 -> get i5 (set i5 z1 t1) = z1.
+         i5 < len t1 -> get i5 (set i5 z1 t1) = z1.
 
 Axiom get_set_neq: 
   forall (a7 : Type) (t2:array a7) (i6:int)(j:int) (z2:a7),
-    i6 < length t2 -> j < length t2 ->
+    i6 < len t2 -> j < len t2 ->
        i6 <> j -> get i6 (set j z2 t2) = get i6 t2.
 
-Axiom length_nonnegative: 
-  forall (a8 : Type) (t3:array a8), 0 <= length t3.  
+Axiom len_nonnegative: 
+  forall (a8 : Type) (t3:array a8), 0 <= len t3.  
