hashtbl/add_who.v
@@ -12,28 +12,23 @@ Section sec. (*who*)
                    kmap.  (*who*) Admitted.
   (*whorestrict*) Definition restrict: forall   (e11 e21 : kmap), kmap ->
                     kmap.  (*who*) Admitted.
-  (*whoLis*) Require Import WhoList. (*who*) 
   (*whoArra*) Require Import WhoArray. (*who*) 
-  (*whohashkey*) Definition hashkey : Type.  (*who*) Admitted.
-  (*whohash*) Definition hash: hashkey -> int.  (*who*) 
-  Admitted.
-  (*whorepr*) Definition repr: forall (b : Type)  , (array (list (hashkey *
-                b))) -> (list (hashkey * b)) -> Prop.  (*who*) 
-  Admitted.
-  (*whoa*) Variables a : Type. Variables r : key.  (*who*) 
-  (*whol*) Variable l: list (hashkey * a).  (*who*) 
-  (*whoh*) Variable h: ref (array (list (hashkey * a))) r.  (*who*) 
+  (*whoLis*) Require Import WhoList. (*who*) Admitted.Admitted.Admitted.
+  (*whoHashtb*) Require Import WhoHashtbl. (*who*) (*whoa*) Variables a :
+  Type. Variables r : key.  (*who*) 
+  (*whol*) Variable l: list ((hashkey) * a).  (*who*) 
+  (*whoh*) Variable h: ref (array (list ((hashkey) * a))) r.  (*who*) 
   (*whokey*) Variable key: hashkey.  (*who*) 
   (*whos*) Variable s: kmap.  (*who*) (*whoval*) Variable val: a.  (*who*) 
-  (*whoH*) Hypothesis H: 0 < (length (!! h s)).  (*who*) 
+  (*whoH*) Hypothesis H: 0 < (len (!! h s)).  (*who*) 
   (*whoH1*) Hypothesis H1:
             forall (i1:int),
             (0 <= i1) ->
-            ((i1 < (length (!! h s))) ->
+            ((i1 < (len (!! h s))) ->
              (forall (k1:hashkey),
               forall (v1:a),
               (l_in (k1 , v1) (get i1 (!! h s))) ->
-              ((mod (hash k1) (length (!! h s))) = i1))).  (*who*) 
+              ((mod (hash k1) (len (!! h s))) = i1))).  (*who*) 
   (*whoH2*) Hypothesis H2: repr (!! h s) l.  (*who*) 
   (*whos1*) Variable s1: kmap.  (*who*) 
   (*whoH3*) Hypothesis H3: (!! h s) = (!! h s1).  (*who*) 
@@ -44,20 +39,20 @@ Section sec. (*who*)
   (*whos4*) Variable s4: kmap.  (*who*) 
   (*whoH6*) Hypothesis H6:
             (!! h s4) =
-            (set (mod (hash key) (length (!! h s1)))
+            (set (mod (hash key) (len (!! h s1)))
              (cons (key , val)
-              (get (mod (hash key) (length (!! h s1))) (!! h s2)))
+              (get (mod (hash key) (len (!! h s1))) (!! h s2)))
              (!! h s3)).  (*who*) 
-  (*whogoal*) Lemma goal: 0 < (length (!! h s4)). (*who*) 
+  (*whogoal*) Lemma goal: 0 < (len (!! h s4)). (*who*) 
   Proof.  rewrite H6, <- update_length, <- H5, <- H4, <- H3. auto. Qed.
   (*whobeginsec1*)
   Section sec1. (*who*)
     (*whoi*) Variable i: int.  (*who*) 
     (*whoH7*) Hypothesis H7: 0 <= i.  (*who*) 
-    (*whoH8*) Hypothesis H8: i < (length (!! h s4)).  (*who*) 
+    (*whoH8*) Hypothesis H8: i < (len (!! h s4)).  (*who*) 
     (*whok*) Variable k: hashkey.  (*who*) (*whov*) Variable v: a.  (*who*) 
     (*whoH9*) Hypothesis H9: l_in (k , v) (get i (!! h s4)).  (*who*) 
-    (*whogoal1*) Lemma goal1: (mod (hash k) (length (!! h s4))) = i. (*who*) 
+    (*whogoal1*) Lemma goal1: (mod (hash k) (len (!! h s4))) = i. (*who*) 
     Proof.
       rewrite H6, H3, H4, H5 in *|-*; rewrite <- update_length in *|-*; clear H6 H5 H4 H3.
       case_eq (Z_eq_dec i (mod (hash key) (length (!! h s3)))); intros; auto.
